some progress on bv_tac for abstract U64 etc.

examples/tactics/TestBV.fst
@@ -5,30 +5,43 @@ open FStar.Tactics
 open FStar.Tactics.BV
 
 let test1 (x y: uint_t 64) =
-    assert_by_tactic (logand #64 x y == logand #64 y x)
+    assert_by_tactic (logand x y == logand y x)
                      (bv_tac ())
 
 let test2 (x y : uint_t 64) = 
-    assert_by_tactic (logand #64 (logand #64 x y) y == logand #64 y (logand #64 y x))
+    assert_by_tactic (logand (logand x y) y == logand y (logand y x))
                      (bv_tac ())
 
 let test3 (x y : uint_t 64) = 
-    assert_by_tactic (logand #64 (logand #64 (logand #64 x y) x) y == logand #64 y (logand #64 x (logand #64 y x)))
+    assert_by_tactic (logand (logand (logand x y) x) y == logand y (logand x (logand y x)))
                      (bv_tac ())
 
 let test4 (x y : uint_t 64) = 
-    assert_by_tactic (logand #64 (logand #64 x (logxor #64 x y)) y == logand #64 y (logand #64 x (logxor #64 y x)))
+    assert_by_tactic (logand (logand x (logxor x y)) y == logand y (logand x (logxor y x)))
                      (bv_tac ())
 
 module U64 = FStar.UInt64
 let test5 (x y: U64.t) =
-    assert_by_tactic (logand #64 (U64.v x) (U64.v y) == logand #64 (U64.v y) (U64.v x))
+    assert_by_tactic (logand (U64.v x) (U64.v y) == logand (U64.v y) (U64.v x))
                      (bv_tac ())
 
 let unfold_logand64 (x y: U64.t) : Lemma 
   (U64.v (U64.logand x y) == logand #64 (U64.v x) (U64.v y))
   = ()
 
+let unfold_logor64 (x y: U64.t) : Lemma 
+  (U64.v (U64.logor x y) == logor #64 (U64.v x) (U64.v y))
+  = ()
+
+let unfold_logxor64 (x y: U64.t) : Lemma 
+  (U64.v (U64.logxor x y) == logxor #64 (U64.v x) (U64.v y))
+  = ()
+
+let unfold64 () = 
+  or_else (apply_lemma (quote unfold_logand64))
+          (or_else (apply_lemma (quote unfold_logor64))
+                   (or_else (apply_lemma (quote unfold_logxor64))
+                           idtac))
 
 let v64_eq (x y: U64.t) : Lemma 
   (requires (U64.v x == U64.v y))
@@ -43,28 +56,22 @@ let trans (a:Type)
         : Lemma (w == z)
         = ()
 
-let bv_tac ()  =
-  apply_lemma (quote eq_to_bv);;
-  apply_lemma (quote FStar.Tactics.BV.trans);;
-  arith_to_bv_tac;;
-  arith_to_bv_tac;;
-  set_options "--smtencoding.elim_box true";;
-  dump "BEFORE SMT!" ;;
-  smt
+// let bv64_tac ()  =
+//   apply_lemma (quote eq_to_bv);;
+//   apply_lemma (quote FStar.Tactics.BV.trans);;
+//   arith_to_bv_tac;;
+//   arith_to_bv_tac;;
+//   set_options "--smtencoding.elim_box true";;
+//   norm [delta];;
+//   fail #unit "BEFORE SMT!" ;;
+//   smt
 
-// let test6 (x y: U64.t) =
-//     assert_by_tactic (U64.logand x y == U64.logand y x)
-//                      (apply_lemma (quote v64_eq) ;;
-//                       dump "A" ;;
-//                       apply_lemma (quote trans) ;; 
-//                       apply_lemma (quote unfold_logand64) ;;
-//                       dump "B";;
-//                       apply_lemma (quote unfold_logand64) ;;
-//                       dump "C";;
-//                       norm [] ;;
-//                       bv_tac ())
-                     
-// //cannot prove
-// (* let test5 (x : uint_t 32) = *)
-// (*     assert_by_tactic (shift_left #32 x 3 == shift_left #32 (shift_left #32 x 2) 1) *)
-// (*                      (prune "";; addns "Prims";; bv_tac ()) *)
+//#reset-options "--log_queries --z3refresh"
+let test6 (x y: U64.t) =
+    assert_by_tactic (U64.logand x y == U64.logand y x)
+                     (apply_lemma (quote v64_eq) ;;
+                      apply_lemma (quote trans) ;; 
+                      unfold64 () ;; unfold64() ;;
+                      norm [] ;;
+                      bv_tac ())
+
